add deep embedding semantics

HeapLang/WeakestPrecondition.thy
@@ -6,28 +6,28 @@ subsection \<open>Weakest Preconditions\<close>
 text \<open>
   The functions below mirror the stepwise derivation of wp from "Iris from ground up".
 \<close>
-function wp1 :: "expr \<Rightarrow> (val \<Rightarrow> ('a::ucamera) iprop) \<Rightarrow> 'a iprop" where
+function wp1 :: "expr \<Rightarrow> (val \<Rightarrow> iprop) \<Rightarrow> iprop" where
   "wp1 e \<Phi> = (case to_val e of Some v \<Rightarrow> \<Phi> v 
     | None \<Rightarrow> (\<forall>\<^sub>u \<sigma>. ((\<upharpoonleft>(red e \<sigma>)) \<and>\<^sub>u \<triangleright>(\<forall>\<^sub>u \<kappa> e2 \<sigma>2. (\<upharpoonleft>(e \<sigma> \<kappa> \<Rightarrow>\<^sub>h e2 \<sigma>2 [])) -\<^emph> wp1 e2 \<Phi>))))"
     by fastforce blast
 
-definition own_state_heap :: "state \<Rightarrow> 'a::ucamera heapGCmra iprop" where
+definition own_state_heap :: "state \<Rightarrow> iprop" where
   "own_state_heap s = Own\<^sub>h (full (to_heap_op (heap s)))"
 
-function wp2 :: "expr \<Rightarrow> (val \<Rightarrow> 'a::ucamera heapGCmra iprop) \<Rightarrow> 'a heapGCmra iprop" where
+function wp2 :: "expr \<Rightarrow> (val \<Rightarrow> iprop) \<Rightarrow> iprop" where
   "wp2 e \<Phi> = (case to_val e of Some v \<Rightarrow> \<Rrightarrow>\<^sub>b (\<Phi> v)
     | None \<Rightarrow> (\<forall>\<^sub>u \<sigma>. (own_state_heap \<sigma> -\<^emph>
       \<Rrightarrow>\<^sub>b ((\<upharpoonleft>(red e \<sigma>)) \<and>\<^sub>u \<triangleright>(\<forall>\<^sub>u \<kappa> e2 \<sigma>2. (\<upharpoonleft>(e \<sigma> \<kappa> \<Rightarrow>\<^sub>h e2 \<sigma>2 [])) -\<^emph> 
         \<Rrightarrow>\<^sub>b ((own_state_heap \<sigma>2) \<^emph> wp2 e2 \<Phi>))))))"
    by fast simp
 
-function wp3 :: "expr \<Rightarrow> (val \<Rightarrow> 'a::ucamera heapGCmra iprop) \<Rightarrow> 'a heapGCmra iprop" where
+function wp3 :: "expr \<Rightarrow> (val \<Rightarrow> iprop) \<Rightarrow> iprop" where
   "wp3 e \<Phi> = (case to_val e of Some v \<Rightarrow> \<Rrightarrow>\<^sub>b (\<Phi> v)
     | None \<Rightarrow> (\<forall>\<^sub>u \<sigma>. (own_state_heap \<sigma> -\<^emph>
       \<Rrightarrow>\<^sub>b ((\<upharpoonleft>(red e \<sigma>)) \<and>\<^sub>u \<triangleright>(\<forall>\<^sub>u \<kappa> e2 \<sigma>2 efs. (\<upharpoonleft>(e \<sigma> \<kappa> \<Rightarrow>\<^sub>h e2 \<sigma>2 efs)) -\<^emph> 
         \<Rrightarrow>\<^sub>b ((own_state_heap \<sigma>2) \<^emph> wp3 e2 \<Phi> \<^emph> (sep_map_set (\<lambda>e'. wp3 e' (\<lambda>_. \<upharpoonleft>True)) (set efs))))))))"
   by fast auto
 
-abbreviation wp :: "expr \<Rightarrow> (val \<Rightarrow> 'a::ucamera heapGCmra iprop) \<Rightarrow> 'a heapGCmra iprop" where 
+abbreviation wp :: "expr \<Rightarrow> (val \<Rightarrow> iprop) \<Rightarrow> iprop" where 
   "wp \<equiv> wp3"
 end
