IrisCore/BaseLogicDeep.thy
@@ -27,12 +27,91 @@ inductive judgement :: "(string\<times>logic_type) list \<Rightarrow> 'a::ucamer
 | ExistsE: "(x,\<tau>)#\<Gamma>|P\<turnstile>Q \<Longrightarrow> \<Gamma>|Exists x \<tau> P\<turnstile>Q"
 | EtaRed: "I|P\<turnstile>Q \<Longrightarrow> I|P\<turnstile>Abs x \<tau> (AppL Q (VarL x))"
 
-
 datatype 'a semantic_type = PropS "'a \<Rightarrow> nat \<Rightarrow> bool" | CmraS 'a | UnitS unit 
-  | SumS "'a semantic_type + 'a semantic_type" | ProdT "'a semantic_type\<times>'a semantic_type" 
-  | FunT "'a semantic_type fset"
-  | Expr expr | State state | Observation observation | List "'a semantic_type list"
+  | SumS "'a semantic_type + 'a semantic_type" | ProdS "'a semantic_type\<times>'a semantic_type" 
+  | FunS "('a semantic_type\<times>'a semantic_type) fset" \<comment> \<open>BNFs can't have recursion in function arguments\<close>
+  | ExprS expr | StateS state | ObservationS observation | ListS "'a semantic_type list"
 
-fun logic_semantic :: "'a::ucamera logic_term \<Rightarrow> 'a semantic_type" where
-  "logic_semantic Unit = UnitS ()"
+definition funS :: "('a semantic_type\<Rightarrow>'a semantic_type) \<Rightarrow> 'a semantic_type" where
+  "funS f = FunS (Abs_fset {(x,y) | x y. f x = y})"
+
+definition appS :: "'a semantic_type \<Rightarrow> 'a semantic_type \<Rightarrow> 'a semantic_type" where
+  "appS fS x \<equiv> case fS of FunS f \<Rightarrow> the_elem ((fset f) `` {x}) | _ \<Rightarrow> undefined"
+notation appS (infixl "$$" 60)
+
+abbreviation "unwrap_expr eS \<equiv> case eS of ExprS e \<Rightarrow> e | _ \<Rightarrow> undefined"
+abbreviation "unwrap_state sS \<equiv> case sS of StateS s \<Rightarrow> s | _ \<Rightarrow> undefined"
+abbreviation "unwrap_obs oS \<equiv> case oS of ObservationS ob \<Rightarrow> ob | _ \<Rightarrow> undefined"
+abbreviation "unwrap_list m lS \<equiv> case lS of ListS l \<Rightarrow> map m l | _ \<Rightarrow> undefined"
+abbreviation "unwrap_prop pS x n \<equiv> case pS of PropS p \<Rightarrow> p x n | _ \<Rightarrow> undefined"
+
+definition head_step_sem :: "'a::ucamera semantic_type" where
+  "head_step_sem \<equiv> funS (\<lambda>e1S. funS (\<lambda>s1S. funS (\<lambda>kl. funS (\<lambda>e2S. funS (\<lambda>s2S. funS (\<lambda>efsl. 
+      PropS (\<lambda>_ _.
+      ((unwrap_expr e1S) (unwrap_state s1S) (unwrap_list unwrap_obs kl) \<Rightarrow>\<^sub>h 
+      (unwrap_expr e2S) (unwrap_state s2S) (unwrap_list unwrap_expr efsl))
+  )))))))"
+
+definition "wp_sem \<equiv> funS 
+  (\<lambda>e. PropS (\<lambda>x n. \<forall>s1 k e2 s2 efs. unwrap_prop (head_step_sem$$e$$s1$$k$$e2$$s2$$efs) x n))"
+
+abbreviation "comb_prop p q pcomb \<equiv> (case p of Some (PropS p') \<Rightarrow> (case q of Some (PropS q') \<Rightarrow> 
+  Some (PropS (\<lambda>a n. pcomb p' q' a n)) | _ \<Rightarrow> None) | _ \<Rightarrow> None)"
+  
+fun logic_semantic 
+  :: "'a::ucamera logic_term \<Rightarrow> (string\<rightharpoonup>'a semantic_type) \<Rightarrow> 'a semantic_type option" where
+  "logic_semantic Unit _ = Some (UnitS ())"
+| "logic_semantic (VarL v) \<Gamma> = \<Gamma> v"
+| "logic_semantic (Prod f s) \<Gamma> = comb_option (logic_semantic f \<Gamma>) (logic_semantic s \<Gamma>) 
+  (\<lambda>fS sS. ProdS (fS,sS))"
+| "logic_semantic (FstL p) \<Gamma> = (case logic_semantic p \<Gamma> of Some (ProdS pS) \<Rightarrow> Some (fst pS) 
+  | _ \<Rightarrow> None)"
+| "logic_semantic (SndL p) \<Gamma> = (case logic_semantic p \<Gamma> of Some (ProdS pS) \<Rightarrow> Some (snd pS) 
+  | _ \<Rightarrow> None)"
+| "logic_semantic (Abs v _ b) \<Gamma> = Some (funS (\<lambda>vS. the (logic_semantic b (\<Gamma>(v\<mapsto>vS)))))"
+| "logic_semantic (AppL f x) \<Gamma> = comb_option (logic_semantic f \<Gamma>) (logic_semantic x \<Gamma>) appS"
+| "logic_semantic (Const x) _ = Some (CmraS x)"
+| "logic_semantic (Core x) \<Gamma> = (case logic_semantic x \<Gamma> of Some (CmraS x') \<Rightarrow> Some (CmraS (core x')) 
+  | _ \<Rightarrow> None)"
+| "logic_semantic (Comp x y) \<Gamma> = (case logic_semantic x \<Gamma> of Some (CmraS x') \<Rightarrow> 
+  (case logic_semantic y \<Gamma> of Some (CmraS y') \<Rightarrow> Some (CmraS (x'\<cdot>y')) | _ \<Rightarrow> None) | _ \<Rightarrow> None)"
+| "logic_semantic FalseTrm _ = Some (PropS (\<lambda>_ _. False))"
+| "logic_semantic TrueTrm _ = Some (PropS (\<lambda>_ _. True))"
+| "logic_semantic (EqTrm _ x y) \<Gamma> = comb_option (logic_semantic x \<Gamma>) (logic_semantic y \<Gamma>) 
+  (\<lambda>x y. PropS (\<lambda> _ _. x=y))"
+| "logic_semantic (Impl p q) \<Gamma> = comb_prop (logic_semantic p \<Gamma>) (logic_semantic q \<Gamma>) 
+  (\<lambda>p q a n. p a n \<longrightarrow> q a n)"
+| "logic_semantic (Conj p q) \<Gamma> = comb_prop (logic_semantic p \<Gamma>) (logic_semantic q \<Gamma>) 
+  (\<lambda>p q a n. p a n \<and> q a n)"
+| "logic_semantic (Disj p q) \<Gamma> = comb_prop (logic_semantic p \<Gamma>) (logic_semantic q \<Gamma>) 
+  (\<lambda>p q a n. p a n \<or> q a n)"
+| "logic_semantic (Sep p q) \<Gamma> = comb_prop (logic_semantic p \<Gamma>) (logic_semantic q \<Gamma>) 
+  (\<lambda>p q a n. \<exists>b1 b2. n_equiv n a (b1\<cdot>b2) \<and> p b1 n \<and> q b2 n)"
+| "logic_semantic (Wand p q) \<Gamma> = comb_prop (logic_semantic p \<Gamma>) (logic_semantic q \<Gamma>) 
+  (\<lambda>p q a n. \<forall>b m. m\<le>n \<longrightarrow> n_valid (a \<cdot> b) m \<longrightarrow> p b m \<longrightarrow> q (a \<cdot> b) m)"
+| "logic_semantic (Guarded v _ b) \<Gamma> = (if guarded v b then 
+  Some (funS (\<lambda>vS. the (logic_semantic b (\<Gamma>(v\<mapsto>vS))))) else None)"
+| "logic_semantic (Exists v _ b) \<Gamma> = 
+  Some (PropS (\<lambda>a n. \<exists>vS. unwrap_prop (the (logic_semantic b (\<Gamma>(v\<mapsto>vS)))) a n))"
+| "logic_semantic (Forall v _ b) \<Gamma> = 
+  Some (PropS (\<lambda>a n. \<forall>vS. unwrap_prop (the (logic_semantic b (\<Gamma>(v\<mapsto>vS)))) a n))"
+| "logic_semantic (Own x) \<Gamma> = (case logic_semantic x \<Gamma> of Some (CmraS x') \<Rightarrow> 
+  Some (PropS (\<lambda>a n. n_incl n x' a)) | _ \<Rightarrow> None)"
+| "logic_semantic (Valid x) \<Gamma> = (case logic_semantic x \<Gamma> of Some (CmraS x') \<Rightarrow> 
+  Some (PropS (\<lambda>_. n_valid x')) | _ \<Rightarrow> None)"
+| "logic_semantic (Persistent p) \<Gamma> = (case logic_semantic p \<Gamma> of Some (PropS p') \<Rightarrow> 
+  Some (PropS (\<lambda>a n. p' (core a) n)) | _ \<Rightarrow> None)"
+| "logic_semantic (Plain p) \<Gamma> = (case logic_semantic p \<Gamma> of Some (PropS p') \<Rightarrow>
+  Some (PropS (\<lambda>_ n. p' \<epsilon> n)) | _ \<Rightarrow> None)"
+| "logic_semantic (Later p) \<Gamma> = (case logic_semantic p \<Gamma> of Some (PropS p') \<Rightarrow>
+  Some (PropS (\<lambda>a n. n=0 \<or> p' a (n-1))))"
+| "logic_semantic (Upd p) \<Gamma> = (case logic_semantic p \<Gamma> of Some (PropS p') \<Rightarrow>
+  Some (PropS (\<lambda>a n. \<forall>m b. m\<le>n \<longrightarrow> n_valid (a \<cdot> b) m \<longrightarrow> (\<exists>c. n_valid (c \<cdot> b) m \<and> p' c m))))"
+
+lemma "types_of_term t \<Gamma>T = None \<Longrightarrow> logic_semantic t \<Gamma>S = None"
+sorry  
+
+lemma "logic_semantic wp [''head_step''\<mapsto>head_step_sem] = Some wp_sem"
+apply (simp add: wp_def head_step_sem_def funS_def appS_def the_elem_def Abs_fset_inverse)
+sorry
 end
